slabs bottom-up 30/n: size class alloc
remaining:
- tons of admit/assume
- vrefine over size_class
- size_class selection
- init

src/SizeClass.fst
@@ -22,11 +22,324 @@ open Slabs
 //TODO: use ptrdiff
 //assume val f (md: slab_metadata) : arr:array U8.t{A.length arr = U32.v page_size}
 
-(*)
-(*)
 // Given a size, return a size_class
 // TODO: improve max_sc bound
 // (requires an improved Steel while loop)
+
+
+noeq
+type size_class_struct = {
+  size: sc;
+  partial_slabs: ref (SL.t blob);
+  empty_slabs: ref (SL.t blob);
+  region_start: array (arr:array U8.t{A.length arr = U32.v page_size});
+  lock: ref bool;
+  metadata_allocated: U32.t;
+}
+
+noeq
+type blob2 = {
+  scs_v: size_class_struct;
+  partial_slabs_v: list blob;
+  empty_slabs_v: list blob;
+}
+
+let size_class_sl'
+  (r: ref size_class_struct)
+  (scs: size_class_struct)
+  : Mem.slprop u#1
+  =
+  pts_to_sl r full_perm scs `Mem.star`
+  SL.ind_llist_sl (p_partial scs.size) (scs.partial_slabs) `Mem.star`
+  SL.ind_llist_sl (p_empty scs.size) (scs.empty_slabs)
+
+let size_class_sl
+  (r: ref size_class_struct)
+  =
+  Mem.h_exists (size_class_sl' r)
+
+let size_class_sl'_witinv (r: ref size_class_struct)
+  : Lemma (Mem.is_witness_invariant (size_class_sl' r))
+  =
+  let aux (scs1 scs2: size_class_struct) (m: Mem.mem)
+  : Lemma
+  (requires
+    Mem.interp (size_class_sl' r scs1) m /\
+    Mem.interp (size_class_sl' r scs2) m
+  )
+  (ensures scs1 == scs2)
+  =
+  pts_to_witinv r full_perm;
+  assert (scs1 == scs2);
+  pts_to_witinv (scs1.partial_slabs) full_perm;
+  pts_to_witinv (scs1.empty_slabs) full_perm
+  in
+  Classical.forall_intro_3 (Classical.move_requires_3 aux)
+
+let size_class_sel_full'
+  (r: ref size_class_struct)
+  : selector' blob2 (size_class_sl r)
+  =
+  fun (h:_) ->
+    let scs : size_class_struct = G.reveal (Mem.id_elim_exists (size_class_sl' r) h) in
+    assert (Mem.interp (size_class_sl' r scs) h);
+    let p1 = pts_to_sl r full_perm scs in
+    let p2 = SL.ind_llist_sl (p_partial scs.size) scs.partial_slabs in
+    let p3 = SL.ind_llist_sl (p_empty scs.size) scs.empty_slabs in
+    let sl = p1 `Mem.star` p2 `Mem.star` p3 in
+    assert (Mem.interp sl h);
+    let partial_slabs_v = SL.ind_llist_sel (p_partial scs.size) scs.partial_slabs h in
+    let empty_slabs_v = SL.ind_llist_sel (p_empty scs.size) scs.empty_slabs h in
+    let b = {
+      scs_v = G.reveal scs;
+      partial_slabs_v = partial_slabs_v;
+      empty_slabs_v = empty_slabs_v;
+    } in
+    b
+
+let size_class_sel_depends_only_on
+  (r: ref size_class_struct)
+  (m0:Mem.hmem (size_class_sl r)) (m1:Mem.mem{Mem.disjoint m0 m1})
+  : Lemma
+  (size_class_sel_full' r m0 == size_class_sel_full' r (Mem.join m0 m1))
+  =
+  let m' = Mem.join m0 m1 in
+  let b1 = G.reveal (Mem.id_elim_exists (size_class_sl' r) m0) in
+  let b2 = G.reveal (Mem.id_elim_exists (size_class_sl' r) m') in
+  size_class_sl'_witinv r;
+  Mem.elim_wi (size_class_sl' r) b1 b2 m'
+
+let size_class_sel_depends_only_on_core
+  (r: ref size_class_struct)
+  (m0:Mem.hmem (size_class_sl r))
+  : Lemma
+  (size_class_sel_full' r m0 == size_class_sel_full' r (Mem.core_mem m0))
+  =
+  let b1 = G.reveal (Mem.id_elim_exists (size_class_sl' r) m0) in
+  let b2 = G.reveal (Mem.id_elim_exists (size_class_sl' r) (Mem.core_mem m0)) in
+  size_class_sl'_witinv r;
+  Mem.elim_wi (size_class_sl' r) b1 b2 (Mem.core_mem m0)
+
+let size_class_sel (r: ref size_class_struct)
+  : selector blob2 (size_class_sl r)
+  =
+  Classical.forall_intro_2 (size_class_sel_depends_only_on r);
+  Classical.forall_intro (size_class_sel_depends_only_on_core r);
+  size_class_sel_full' r
+
+[@@ __steel_reduce__]
+let size_class_full' (r: ref size_class_struct) : vprop'
+  = {
+    hp = size_class_sl r;
+    t = blob2;
+    sel = size_class_sel r;
+  }
+unfold
+let size_class_full (r: ref size_class_struct) = VUnit (size_class_full' r)
+
+[@@ __steel_reduce__]
+let v_sc_full (#p: vprop) (r: ref size_class_struct)
+  (h: rmem p{FStar.Tactics.with_tactic selector_tactic (can_be_split p (size_class_full r) /\ True)})
+  = h (size_class_full r)
+
+let unpack_sc_lemma
+  (r: ref size_class_struct)
+  (b: blob2)
+  (m: Mem.mem)
+  : Lemma
+  (requires
+    Mem.interp (size_class_sl r) m /\
+    size_class_sel r m == b
+  )
+  (ensures (
+    Mem.interp (
+      SR.ptr r `Mem.star`
+      SL.ind_llist_sl (p_partial b.scs_v.size) b.scs_v.partial_slabs `Mem.star`
+      SL.ind_llist_sl (p_empty b.scs_v.size) b.scs_v.empty_slabs
+    ) m /\
+    sel_of (vptr r) m == b.scs_v /\
+    SL.ind_llist_sel (p_partial b.scs_v.size) b.scs_v.partial_slabs m == b.partial_slabs_v /\
+    SL.ind_llist_sel (p_empty b.scs_v.size) b.scs_v.empty_slabs m == b.empty_slabs_v /\
+    True
+  ))
+  =
+  let p1 = pts_to_sl r full_perm b.scs_v in
+  let p2 = SL.ind_llist_sl (p_partial b.scs_v.size) b.scs_v.partial_slabs in
+  let p3 = SL.ind_llist_sl (p_empty b.scs_v.size) b.scs_v.empty_slabs in
+  let sl = p1 `Mem.star` p2 `Mem.star` p3 in
+  assert (Mem.interp sl m);
+
+  let m12, m3 = Mem.id_elim_star (p1 `Mem.star` p2) p3 m in
+  let m1, m2 = Mem.id_elim_star p1 p2 m12 in
+  // #1
+  intro_ptr_interp r b.scs_v m1;
+  ptr_sel_interp r m1;
+  pts_to_witinv r full_perm;
+  // #2
+  // #3
+  //
+  Mem.intro_star
+    (SR.ptr r) p2 m1 m2;
+  assert (G.reveal m12 == Mem.join m1 m2);
+  Mem.intro_star
+    (SR.ptr r `Mem.star` p2) p3 m12 m3;
+  assert (m == Mem.join m12 m3);
+  ()
+
+let unpack_sc (r: ref size_class_struct)
+  : Steel size_class_struct
+  (size_class_full r)
+  (fun scs ->
+    vptr r `star`
+    SL.ind_llist (p_partial scs.size) scs.partial_slabs `star`
+    SL.ind_llist (p_empty scs.size) scs.empty_slabs
+  )
+  (requires fun _ -> True)
+  (ensures fun h0 scs h1 ->
+    let b = v_sc_full r h0 in
+    sel r h1 == scs /\
+    sel r h1 == b.scs_v /\
+    SL.v_ind_llist (p_partial scs.size) scs.partial_slabs h1 == b.partial_slabs_v /\
+    SL.v_ind_llist (p_empty scs.size) scs.empty_slabs h1 == b.empty_slabs_v
+  )
+  =
+  let h = get () in
+  let b = G.hide (v_sc_full r h) in
+  change_slprop
+    (size_class_full r)
+    (vptr r `star`
+    SL.ind_llist (p_partial b.scs_v.size) b.scs_v.partial_slabs `star`
+    SL.ind_llist (p_empty b.scs_v.size) b.scs_v.empty_slabs)
+    b
+    ((b.scs_v, b.partial_slabs_v), b.empty_slabs_v)
+    (fun m -> unpack_sc_lemma r (G.reveal b) m);
+  let scs = read r in
+  change_slprop_rel
+    (SL.ind_llist (p_partial b.scs_v.size) b.scs_v.partial_slabs)
+    (SL.ind_llist (p_partial scs.size) scs.partial_slabs)
+    (fun x y -> x == y)
+    (fun _ -> ());
+  change_slprop_rel
+    (SL.ind_llist (p_empty b.scs_v.size) b.scs_v.empty_slabs)
+    (SL.ind_llist (p_empty scs.size) scs.empty_slabs)
+    (fun x y -> x == y)
+    (fun _ -> ());
+  return scs
+
+let pack_sc_lemma
+  (r: ref size_class_struct)
+  (b: blob2)
+  (m: Mem.mem)
+  : Lemma
+  (requires
+    Mem.interp (
+      SR.ptr r `Mem.star`
+      SL.ind_llist_sl (p_partial b.scs_v.size) b.scs_v.partial_slabs `Mem.star`
+      SL.ind_llist_sl (p_empty b.scs_v.size) b.scs_v.empty_slabs
+    ) m /\
+    sel_of (vptr r) m == b.scs_v /\
+    SL.ind_llist_sel (p_partial b.scs_v.size) b.scs_v.partial_slabs m == b.partial_slabs_v /\
+    SL.ind_llist_sel (p_empty b.scs_v.size) b.scs_v.empty_slabs m == b.empty_slabs_v
+  )
+  (ensures
+    Mem.interp (size_class_sl r) m /\
+    size_class_sel r m == b
+  )
+  =
+  let p1 = SR.ptr r in
+  let p2 = SL.ind_llist_sl (p_partial b.scs_v.size) b.scs_v.partial_slabs in
+  let p3 = SL.ind_llist_sl (p_empty b.scs_v.size) b.scs_v.empty_slabs in
+  let sl = p1 `Mem.star` p2 `Mem.star` p3 in
+  assert (Mem.interp sl m);
+
+  let m12, m3 = Mem.id_elim_star (p1 `Mem.star` p2) p3 m in
+  let m1, m2 = Mem.id_elim_star p1 p2 m12 in
+  // #1
+  ptr_sel_interp r m1;
+  let p1' = pts_to_sl r full_perm b.scs_v in
+  // #2
+  // #3
+  //
+  Mem.intro_star p1' p2 m1 m2;
+  Mem.intro_star (p1' `Mem.star` p2) p3 m12 m3;
+  Mem.intro_h_exists b.scs_v (size_class_sl' r) m;
+  size_class_sl'_witinv r
+
+let pack_sc (#opened:_)
+  (r: ref size_class_struct)
+  (scs: size_class_struct)
+  : SteelGhost unit opened
+  (vptr r `star`
+  SL.ind_llist (p_partial scs.size) scs.partial_slabs `star`
+  SL.ind_llist (p_empty scs.size) scs.empty_slabs)
+  (fun _ -> size_class_full r)
+  (requires fun h0 -> sel r h0 == scs)
+  (ensures fun h0 _ h1 ->
+    let b = v_sc_full r h1 in
+    b.scs_v == sel r h0 /\
+    b.scs_v == scs /\
+    b.partial_slabs_v == SL.v_ind_llist (p_partial scs.size) scs.partial_slabs h0 /\
+    b.empty_slabs_v == SL.v_ind_llist (p_empty scs.size) scs.empty_slabs h0
+  )
+  =
+  let h0 = get () in
+  assert (scs == sel r h0);
+  let partial_slabs_v : list blob =
+    G.hide (SL.v_ind_llist (p_partial scs.size) scs.partial_slabs h0) in
+  let empty_slabs_v : list blob =
+    G.hide (SL.v_ind_llist (p_empty scs.size) scs.empty_slabs h0) in
+  let m : G.erased ((size_class_struct * list blob) * list blob) =
+    G.hide ((scs, G.reveal partial_slabs_v), G.reveal empty_slabs_v) in
+  let b : blob2 = G.hide ({
+    scs_v = scs;
+    partial_slabs_v = G.reveal partial_slabs_v;
+    empty_slabs_v = G.reveal empty_slabs_v;
+  }) in
+  change_slprop
+    (vptr r `star`
+    SL.ind_llist (p_partial scs.size) scs.partial_slabs `star`
+    SL.ind_llist (p_empty scs.size) scs.empty_slabs)
+    (size_class_full r)
+    m
+    b
+    (fun m -> pack_sc_lemma r (G.reveal b) m);
+  ()
+
+let temp (r1 r2: ref size_class_struct)
+  : Steel U32.t
+  (size_class_full r1)
+  (fun _ -> size_class_full r1)
+  (requires fun _ -> True)
+  (ensures fun h0 _ h1 ->
+    v_sc_full r1 h0 == v_sc_full r1 h1
+  )
+  =
+  let scs = unpack_sc r1 in
+  pack_sc r1 scs;
+  return 0ul
+
+let allocate_size_class (r: ref size_class_struct)
+  (scs: size_class_struct)
+  : Steel (array U8.t)
+  //(size_class_full r)
+  (vptr r `star`
+  SL.ind_llist (p_partial scs.size) scs.partial_slabs `star`
+  SL.ind_llist (p_empty scs.size) scs.empty_slabs)
+  (fun result ->
+    A.varray result `star`
+    size_class_full r)
+  (requires fun h0 ->
+    sel r h0 == scs /\
+    (Cons? (SL.v_ind_llist (p_partial scs.size) scs.partial_slabs h0) \/
+    Cons? (SL.v_ind_llist (p_empty scs.size) scs.empty_slabs h0)))
+  (ensures fun h0 _ h1 -> True)
+  =
+  //let scs = unpack_sc r in
+  let result = allocate_slab scs.size scs.partial_slabs scs.empty_slabs in
+  pack_sc r scs;
+  return result
+
+(*)
 let select_size_class (size: U32.t)
   : Steel sc
   emp (fun _ -> emp)
@@ -168,296 +481,3 @@ let nb_slots (x: nzn) : nzn = U32.div page_size x
 
 let slab_metadata (size_class: nzn)
   = Seq.lseq bool (U32.v (nb_slots size_class))
-
-
-
-noeq
-type size_class_struct = {
-  size: sc;
-  partial_slabs: ref (SL.t slab_metadata);
-  empty_slabs: ref (SL.t slab_metadata);
-  region_start: array (arr:array U8.t{A.length arr = U32.v page_size});
-  lock: ref bool;
-  metadata_allocated: U32.t;
-}
-
-noeq
-type blob = {
-  scs_v: size_class_struct;
-  partial_slabs_v: list slab_metadata;
-  empty_slabs_v: list slab_metadata;
-}
-
-let size_class_sl'
-  (r: ref size_class_struct)
-  (scs: size_class_struct)
-  : Mem.slprop u#1
-  =
-  pts_to_sl r full_perm scs `Mem.star`
-  SL.ind_llist_sl (p_empty scs.size) (scs.partial_slabs) `Mem.star`
-  SL.ind_llist_sl (p_empty scs.size) (scs.empty_slabs)
-
-let size_class_sl
-  (r: ref size_class_struct)
-  =
-  Mem.h_exists (size_class_sl' r)
-
-let size_class_sl'_witinv (r: ref size_class_struct)
-  : Lemma (Mem.is_witness_invariant (size_class_sl' r))
-  =
-  let aux (scs1 scs2: size_class_struct) (m: Mem.mem)
-  : Lemma
-  (requires
-    Mem.interp (size_class_sl' r scs1) m /\
-    Mem.interp (size_class_sl' r scs2) m
-  )
-  (ensures scs1 == scs2)
-  =
-  pts_to_witinv r full_perm;
-  assert (scs1 == scs2);
-  pts_to_witinv (scs1.partial_slabs) full_perm;
-  pts_to_witinv (scs1.empty_slabs) full_perm
-  in
-  Classical.forall_intro_3 (Classical.move_requires_3 aux)
-
-let size_class_sel_full'
-  (r: ref size_class_struct)
-  : selector' blob (size_class_sl r)
-  =
-  fun (h:_) ->
-    let scs : size_class_struct = reveal (Mem.id_elim_exists (size_class_sl' r) h) in
-    assert (Mem.interp (size_class_sl' r scs) h);
-    let p1 = pts_to_sl r full_perm scs in
-    let p2 = SL.ind_llist_sl (p_empty scs.size) scs.partial_slabs in
-    let p3 = SL.ind_llist_sl (p_empty scs.size) scs.empty_slabs in
-    let sl = p1 `Mem.star` p2 `Mem.star` p3 in
-    assert (Mem.interp sl h);
-    let partial_slabs_v = SL.ind_llist_sel (p_empty scs.size) scs.partial_slabs h in
-    let empty_slabs_v = SL.ind_llist_sel (p_empty scs.size) scs.empty_slabs h in
-    let b = {
-      scs_v = reveal scs;
-      partial_slabs_v = partial_slabs_v;
-      empty_slabs_v = empty_slabs_v;
-    } in
-    b
-
-let size_class_sel_depends_only_on
-  (r: ref size_class_struct)
-  (m0:Mem.hmem (size_class_sl r)) (m1:Mem.mem{Mem.disjoint m0 m1})
-  : Lemma
-  (size_class_sel_full' r m0 == size_class_sel_full' r (Mem.join m0 m1))
-  =
-  let m' = Mem.join m0 m1 in
-  let b1 = reveal (Mem.id_elim_exists (size_class_sl' r) m0) in
-  let b2 = reveal (Mem.id_elim_exists (size_class_sl' r) m') in
-  size_class_sl'_witinv r;
-  Mem.elim_wi (size_class_sl' r) b1 b2 m'
-
-let size_class_sel_depends_only_on_core
-  (r: ref size_class_struct)
-  (m0:Mem.hmem (size_class_sl r))
-  : Lemma
-  (size_class_sel_full' r m0 == size_class_sel_full' r (Mem.core_mem m0))
-  =
-  let b1 = reveal (Mem.id_elim_exists (size_class_sl' r) m0) in
-  let b2 = reveal (Mem.id_elim_exists (size_class_sl' r) (Mem.core_mem m0)) in
-  size_class_sl'_witinv r;
-  Mem.elim_wi (size_class_sl' r) b1 b2 (Mem.core_mem m0)
-
-let size_class_sel (r: ref size_class_struct)
-  : selector blob (size_class_sl r)
-  =
-  Classical.forall_intro_2 (size_class_sel_depends_only_on r);
-  Classical.forall_intro (size_class_sel_depends_only_on_core r);
-  size_class_sel_full' r
-
-[@@ __steel_reduce__]
-let size_class_full' (r: ref size_class_struct) : vprop'
-  = {
-    hp = size_class_sl r;
-    t = blob;
-    sel = size_class_sel r;
-  }
-unfold
-let size_class_full (r: ref size_class_struct) = VUnit (size_class_full' r)
-
-[@@ __steel_reduce__]
-let v_sc_full (#p: vprop) (r: ref size_class_struct)
-  (h: rmem p{FStar.Tactics.with_tactic selector_tactic (can_be_split p (size_class_full r) /\ True)})
-  = h (size_class_full r)
-
-let unpack_sc_lemma
-  (r: ref size_class_struct)
-  (b: blob)
-  (m: Mem.mem)
-  : Lemma
-  (requires
-    Mem.interp (size_class_sl r) m /\
-    size_class_sel r m == b
-  )
-  (ensures (
-    Mem.interp (
-      SR.ptr r `Mem.star`
-      SL.ind_llist_sl (p_empty b.scs_v.size) b.scs_v.partial_slabs `Mem.star`
-      SL.ind_llist_sl (p_empty b.scs_v.size) b.scs_v.empty_slabs
-    ) m /\
-    sel_of (vptr r) m == b.scs_v /\
-    SL.ind_llist_sel (p_empty b.scs_v.size) b.scs_v.partial_slabs m == b.partial_slabs_v /\
-    SL.ind_llist_sel (p_empty b.scs_v.size) b.scs_v.empty_slabs m == b.empty_slabs_v /\
-    True
-  ))
-  =
-  let p1 = pts_to_sl r full_perm b.scs_v in
-  let p2 = SL.ind_llist_sl (p_empty b.scs_v.size) b.scs_v.partial_slabs in
-  let p3 = SL.ind_llist_sl (p_empty b.scs_v.size) b.scs_v.empty_slabs in
-  let sl = p1 `Mem.star` p2 `Mem.star` p3 in
-  assert (Mem.interp sl m);
-
-  let m12, m3 = Mem.id_elim_star (p1 `Mem.star` p2) p3 m in
-  let m1, m2 = Mem.id_elim_star p1 p2 m12 in
-  // #1
-  intro_ptr_interp r b.scs_v m1;
-  ptr_sel_interp r m1;
-  pts_to_witinv r full_perm;
-  // #2
-  // #3
-  //
-  Mem.intro_star
-    (SR.ptr r) p2 m1 m2;
-  assert (reveal m12 == Mem.join m1 m2);
-  Mem.intro_star
-    (SR.ptr r `Mem.star` p2) p3 m12 m3;
-  assert (m == Mem.join m12 m3);
-  ()
-
-let unpack_sc (r: ref size_class_struct)
-  : Steel size_class_struct
-  (size_class_full r)
-  (fun scs ->
-    vptr r `star`
-    SL.ind_llist (p_empty scs.size) scs.partial_slabs `star`
-    SL.ind_llist (p_empty scs.size) scs.empty_slabs
-  )
-  (requires fun _ -> True)
-  (ensures fun h0 scs h1 ->
-    let b = v_sc_full r h0 in
-    sel r h1 == scs /\
-    sel r h1 == b.scs_v /\
-    SL.v_ind_llist (p_empty scs.size) scs.partial_slabs h1 == b.partial_slabs_v /\
-    SL.v_ind_llist (p_empty scs.size) scs.empty_slabs h1 == b.empty_slabs_v
-  )
-  =
-  let h = get () in
-  let b = hide (v_sc_full r h) in
-  change_slprop
-    (size_class_full r)
-    (vptr r `star`
-    SL.ind_llist (p_empty b.scs_v.size) b.scs_v.partial_slabs `star`
-    SL.ind_llist (p_empty b.scs_v.size) b.scs_v.empty_slabs)
-    b
-    ((b.scs_v, b.partial_slabs_v), b.empty_slabs_v)
-    (fun m -> unpack_sc_lemma r (reveal b) m);
-  let scs = read r in
-  change_slprop_rel
-    (SL.ind_llist (p_empty b.scs_v.size) b.scs_v.partial_slabs)
-    (SL.ind_llist (p_empty scs.size) scs.partial_slabs)
-    (fun x y -> x == y)
-    (fun _ -> ());
-  change_slprop_rel
-    (SL.ind_llist (p_empty b.scs_v.size) b.scs_v.empty_slabs)
-    (SL.ind_llist (p_empty scs.size) scs.empty_slabs)
-    (fun x y -> x == y)
-    (fun _ -> ());
-  return scs
-
-let pack_sc_lemma
-  (r: ref size_class_struct)
-  (b: blob)
-  (m: Mem.mem)
-  : Lemma
-  (requires
-    Mem.interp (
-      SR.ptr r `Mem.star`
-      SL.ind_llist_sl (p_empty b.scs_v.size) b.scs_v.partial_slabs `Mem.star`
-      SL.ind_llist_sl (p_empty b.scs_v.size) b.scs_v.empty_slabs
-    ) m /\
-    sel_of (vptr r) m == b.scs_v /\
-    SL.ind_llist_sel (p_empty b.scs_v.size) b.scs_v.partial_slabs m == b.partial_slabs_v /\
-    SL.ind_llist_sel (p_empty b.scs_v.size) b.scs_v.empty_slabs m == b.empty_slabs_v
-  )
-  (ensures
-    Mem.interp (size_class_sl r) m /\
-    size_class_sel r m == b
-  )
-  =
-  let p1 = SR.ptr r in
-  let p2 = SL.ind_llist_sl (p_empty b.scs_v.size) b.scs_v.partial_slabs in
-  let p3 = SL.ind_llist_sl (p_empty b.scs_v.size) b.scs_v.empty_slabs in
-  let sl = p1 `Mem.star` p2 `Mem.star` p3 in
-  assert (Mem.interp sl m);
-
-  let m12, m3 = Mem.id_elim_star (p1 `Mem.star` p2) p3 m in
-  let m1, m2 = Mem.id_elim_star p1 p2 m12 in
-  // #1
-  ptr_sel_interp r m1;
-  let p1' = pts_to_sl r full_perm b.scs_v in
-  // #2
-  // #3
-  //
-  Mem.intro_star p1' p2 m1 m2;
-  Mem.intro_star (p1' `Mem.star` p2) p3 m12 m3;
-  Mem.intro_h_exists b.scs_v (size_class_sl' r) m;
-  size_class_sl'_witinv r
-
-let pack_sc (#opened:_)
-  (r: ref size_class_struct)
-  (scs: size_class_struct)
-  : SteelGhost unit opened
-  (vptr r `star`
-  SL.ind_llist (p_empty scs.size) scs.partial_slabs `star`
-  SL.ind_llist (p_empty scs.size) scs.empty_slabs)
-  (fun _ -> size_class_full r)
-  (requires fun h0 -> sel r h0 == scs)
-  (ensures fun h0 _ h1 ->
-    let b = v_sc_full r h1 in
-    b.scs_v == sel r h0 /\
-    b.scs_v == scs /\
-    b.partial_slabs_v == SL.v_ind_llist (p_empty scs.size) scs.partial_slabs h0 /\
-    b.empty_slabs_v == SL.v_ind_llist (p_empty scs.size) scs.empty_slabs h0
-  )
-  =
-  let h0 = get () in
-  assert (scs == sel r h0);
-  let partial_slabs_v : list slab_metadata =
-    hide (SL.v_ind_llist (p_empty scs.size) scs.partial_slabs h0) in
-  let empty_slabs_v : list slab_metadata =
-    hide (SL.v_ind_llist (p_empty scs.size) scs.empty_slabs h0) in
-  let m : erased ((size_class_struct * list slab_metadata) * list slab_metadata) =
-    hide ((scs, reveal partial_slabs_v), reveal empty_slabs_v) in
-  let b : blob = hide ({
-    scs_v = scs;
-    partial_slabs_v = reveal partial_slabs_v;
-    empty_slabs_v = reveal empty_slabs_v;
-  }) in
-  change_slprop
-    (vptr r `star`
-    SL.ind_llist (p_empty scs.size) scs.partial_slabs `star`
-    SL.ind_llist (p_empty scs.size) scs.empty_slabs)
-    (size_class_full r)
-    m
-    b
-    (fun m -> pack_sc_lemma r (reveal b) m);
-  ()
-
-let temp (r1 r2: ref size_class_struct)
-  : Steel U32.t
-  (size_class_full r1)
-  (fun _ -> size_class_full r1)
-  (requires fun _ -> True)
-  (ensures fun h0 _ h1 ->
-    v_sc_full r1 h0 == v_sc_full r1 h1
-  )
-  =
-  let scs = unpack_sc r1 in
-  pack_sc r1 scs;
-  return 0ul
